concurrency/scache/SimpleCache_Refines_AbstractCache.i.dfy
@@ -1,34 +1,291 @@
 include "AbstractCacheSM.i.dfy"
 include "SimpleCacheSM.i.dfy"
+include "SimpleCache_Inv.i.dfy"
 
 module SimpleCache_Refines_AbstractCache refines
     Refinement(CrashAsyncIfc(CacheIfc),
         SimpleCacheStateMachine,
         AbstractCacheStateMachine) {
 
-  predicate Inv(s: A.Variables)
+  import opened SimpleCacheStateMachine
+  import opened RequestIds
+  import SimpleCache_Inv
+
+  predicate Inv(s: A.Variables) {
+    SimpleCache_Inv.Inv(s)
+  }
 
   lemma InitImpliesInv(s: A.Variables)
-  requires A.Init(s)
+  //requires A.Init(s)
   ensures Inv(s)
+  {
+    SimpleCache_Inv.Init_Implies_Inv(s);
+  }
 
   lemma NextPreservesInv(s: A.Variables, s': A.Variables, op: ifc.Op)
-  requires Inv(s)
-  requires A.Next(s, s', op)
+  //requires Inv(s)
+  //requires A.Next(s, s', op)
   ensures Inv(s')
+  {
+    SimpleCache_Inv.Next_PreservesInv(s, s', op);
+  }
+
+  predicate IsInMem(s: Variables, c: nat, d: nat) {
+    c in s.entries && (s.entries[c].Writeback? || s.entries[c].Clean?
+        || s.entries[c].Dirty?)
+      && s.entries[c].disk_idx == d
+  }
+
+
+  predicate InCache(s: Variables, disk_idx: nat) {
+    exists cache_idx :: IsInMem(s, cache_idx, disk_idx)
+  }
+
+  function GetCacheIdx(s: Variables, disk_idx: nat) : nat
+  requires InCache(s, disk_idx)
+  {
+    var cache_idx :| IsInMem(s, cache_idx, disk_idx);
+    cache_idx
+  }
+
+  function GetElem(s: A.Variables, i: nat) : B.Elem
+  requires i in s.disk
+  {
+    B.Elem(s.disk[i],
+      if InCache(s, i) then s.entries[GetCacheIdx(s, i)].data
+          else s.disk[i])
+  }
+
+  function InterpStore(s: A.Variables) : imap<nat, B.Elem>
+  {
+    imap i | i in s.disk :: GetElem(s, i)
+  }
 
   function I(s: A.Variables) : B.Variables
-  requires Inv(s)
+  //requires Inv(s)
+  {
+    B.Variables(
+      InterpStore(s),
+      s.tickets,
+      s.stubs
+    )
+  }
 
   lemma InitRefinesInit(s: A.Variables)
-  requires A.Init(s)
-  requires Inv(s)
+  //requires A.Init(s)
+  //requires Inv(s)
   ensures B.Init(I(s))
+  {
+  }
 
-  lemma NextRefinesNext(s: A.Variables, s': A.Variables, op: ifc.Op)
+  lemma StartRead_Refines(s: Variables, s': Variables, op: ifc.Op, cache_idx: nat, disk_idx: nat)
   requires Inv(s)
   requires Inv(s')
-  requires A.Next(s, s', op)
+  requires StartRead(s, s', op, cache_idx, disk_idx)
   ensures B.Next(I(s), I(s'), op)
+  {
+    assert forall d, c :: IsInMem(s, c, d) <==> IsInMem(s', c, d);
 
+    /*
+    var x := InterpStore(s);
+    var y := InterpStore(s');
+    forall k | k in x
+    ensures k in y && y[k] == x[k]
+    {
+      if InCache(s, k) {
+        assert InCache(s', k);
+        assert GetCacheIdx(s, k) == GetCacheIdx(s', k);
+      }
+      if InCache(s', k) {
+        assert InCache(s, k);
+      }
+      if k == disk_idx {
+        assert k in y && y[k] == x[k];
+      } else {
+        assert k in y && y[k] == x[k];
+      }
+    }
+    assert x == y;
+    */
+
+    assert B.NextStep(I(s), I(s'), op, B.Stutter_Step);
+  }
+
+  lemma FinishRead_Refines(s: Variables, s': Variables, op: ifc.Op, cache_idx: nat, disk_idx: nat) 
+  requires Inv(s)
+  requires FinishRead(s, s', op, cache_idx, disk_idx)
+  requires Inv(s')
+  ensures B.Next(I(s), I(s'), op)
+  {
+    assert forall d, c :: IsInMem(s, c, d) ==> IsInMem(s', c, d);
+    assert forall d, c :: d != disk_idx ==> IsInMem(s', c, d) ==> IsInMem(s, c, d);
+    assert IsInMem(s', cache_idx, disk_idx);
+
+    /*
+    var x := InterpStore(s);
+    var y := InterpStore(s');
+    forall k | k in x
+    ensures k in y && y[k] == x[k]
+    {
+      if k == disk_idx {
+        assert k in y && y[k] == x[k];
+      } else {
+        assert k in y && y[k] == x[k];
+      }
+    }
+    assert x == y;
+    assert I(s) == I(s');
+    */
+    assert B.NextStep(I(s), I(s'), op, B.Stutter_Step);
+  }
+
+  lemma MakeDirty_Refines(s: Variables, s': Variables, op: ifc.Op, cache_idx: nat) 
+  requires Inv(s)
+  requires MakeDirty(s, s', op, cache_idx)
+  requires Inv(s')
+  ensures B.Next(I(s), I(s'), op)
+  {
+    assert forall d, c :: IsInMem(s, c, d) <==> IsInMem(s', c, d);
+    assert B.NextStep(I(s), I(s'), op, B.Stutter_Step);
+  }
+
+  lemma StartWriteback_Refines(s: Variables, s': Variables, op: ifc.Op, cache_idx: nat, disk_idx: nat) 
+  requires Inv(s)
+  requires StartWriteback(s, s', op, cache_idx, disk_idx)
+  requires Inv(s')
+  ensures B.Next(I(s), I(s'), op)
+  {
+    assert forall d, c :: IsInMem(s, c, d) <==> IsInMem(s', c, d);
+    assert B.NextStep(I(s), I(s'), op, B.Stutter_Step);
+  }
+
+  lemma FinishWriteback_Refines(s: Variables, s': Variables, op: ifc.Op, cache_idx: nat, disk_idx: nat) 
+  requires Inv(s)
+  requires FinishWriteback(s, s', op, cache_idx, disk_idx)
+  requires Inv(s')
+  ensures B.Next(I(s), I(s'), op)
+  {
+    assert forall d, c :: IsInMem(s, c, d) <==> IsInMem(s', c, d);
+    assert B.NextStep(I(s), I(s'), op, B.Stutter_Step);
+  }
+
+  lemma Evict_Refines(s: Variables, s': Variables, op: ifc.Op, cache_idx: nat) 
+  requires Inv(s)
+  requires Evict(s, s', op, cache_idx)
+  requires Inv(s')
+  ensures B.Next(I(s), I(s'), op)
+  {
+    assert forall d, c :: IsInMem(s', c, d) ==> IsInMem(s, c, d);
+    assert forall d, c :: c != cache_idx ==> IsInMem(s, c, d) ==> IsInMem(s', c, d);
+    assert IsInMem(s, cache_idx, s.entries[cache_idx].disk_idx);
+
+    assert B.NextStep(I(s), I(s'), op, B.Stutter_Step);
+  }
+
+  lemma ProcessRead_Refines(s: Variables, s': Variables, op: ifc.Op, disk_idx: nat) 
+  requires Inv(s)
+  requires ProcessRead(s, s', op, disk_idx)
+  requires Inv(s')
+  ensures B.Next(I(s), I(s'), op)
+  {
+    assert forall d, c :: IsInMem(s, c, d) <==> IsInMem(s', c, d);
+    assert B.NextStep(I(s), I(s'), op, B.Stutter_Step);
+  }
+
+  lemma ProcessWrite_Refines(s: Variables, s': Variables, op: ifc.Op, disk_idx: nat) 
+  requires Inv(s)
+  requires ProcessWrite(s, s', op, disk_idx)
+  requires Inv(s')
+  ensures B.Next(I(s), I(s'), op)
+  {
+    assert forall d, c :: IsInMem(s, c, d) <==> IsInMem(s', c, d);
+    assert forall c :: SimpleCache_Inv.IsWriter(s, c, disk_idx) ==> IsInMem(s, c, disk_idx);
+    assert disk_idx in InterpStore(s);
+    assert disk_idx in InterpStore(s');
+    assert InterpStore(s')[disk_idx] == B.PersistElem(InterpStore(s)[disk_idx]);
+    assert B.Persist(I(s), I(s'), op, disk_idx);
+    assert B.NextStep(I(s), I(s'), op, B.Persist_Step(disk_idx));
+  }
+
+  lemma Crash_Refines(s: Variables, s': Variables, op: ifc.Op)
+  requires Inv(s)
+  requires Crash(s, s', op)
+  requires Inv(s')
+  ensures B.Next(I(s), I(s'), op)
+  {
+    assert B.NextStep(I(s), I(s'), op, B.Crash_Step);
+  }
+
+  lemma NewTicket_Refines(s: Variables, s': Variables, op: ifc.Op)
+  requires Inv(s)
+  requires NewTicket(s, s', op)
+  requires Inv(s')
+  ensures B.Next(I(s), I(s'), op)
+  {
+    assert forall d, c :: IsInMem(s, c, d) <==> IsInMem(s', c, d);
+    assert B.NextStep(I(s), I(s'), op, B.NewTicket_Step);
+  }
+
+  lemma ConsumeStub_Refines(s: Variables, s': Variables, op: ifc.Op)
+  requires Inv(s)
+  requires ConsumeStub(s, s', op)
+  requires Inv(s')
+  ensures B.Next(I(s), I(s'), op)
+  {
+    assert forall d, c :: IsInMem(s, c, d) <==> IsInMem(s', c, d);
+    assert B.NextStep(I(s), I(s'), op, B.ConsumeStub_Step);
+  }
+
+  lemma ApplyRead_Refines(s: Variables, s': Variables, op: ifc.Op, rid: RequestId, cache_idx: nat) 
+  requires Inv(s)
+  requires ApplyRead(s, s', op, rid, cache_idx)
+  requires Inv(s')
+  ensures B.Next(I(s), I(s'), op)
+  {
+    assert forall d, c :: IsInMem(s, c, d) <==> IsInMem(s', c, d);
+    assert IsInMem(s, cache_idx, s.entries[cache_idx].disk_idx);
+    assert InterpStore(s') == InterpStore(s);
+    assert B.ApplyRead(I(s), I(s'), op, rid);
+    assert B.NextStep(I(s), I(s'), op, B.ApplyRead_Step(rid));
+  }
+
+  lemma ApplyWrite_Refines(s: Variables, s': Variables, op: ifc.Op, rid: RequestId, cache_idx: nat) 
+  requires Inv(s)
+  requires ApplyWrite(s, s', op, rid, cache_idx)
+  requires Inv(s')
+  ensures B.Next(I(s), I(s'), op)
+  {
+    assert forall d, c :: IsInMem(s, c, d) <==> IsInMem(s', c, d);
+    assert IsInMem(s, cache_idx, s.entries[cache_idx].disk_idx);
+    assert B.NextStep(I(s), I(s'), op, B.ApplyWrite_Step(rid));
+  }
+
+  lemma NextStep_Refines(s: Variables, s': Variables, op: ifc.Op, step: Step)
+  requires Inv(s)
+  requires NextStep(s, s', op, step)
+  requires Inv(s')
+  {
+    match step {
+      case StartRead_Step(cache_idx, disk_idx) => { StartRead_Refines(s, s', op, cache_idx, disk_idx); }
+      case FinishRead_Step(cache_idx, disk_idx) => { FinishRead_Refines(s, s', op, cache_idx, disk_idx); }
+      case MakeDirty_Step(cache_idx) => { MakeDirty_Refines(s, s', op, cache_idx); }
+      case StartWriteback_Step(cache_idx, disk_idx) => { StartWriteback_Refines(s, s', op, cache_idx, disk_idx); }
+      case FinishWriteback_Step(cache_idx, disk_idx) => { FinishWriteback_Refines(s, s', op, cache_idx, disk_idx) ; }
+      case Evict_Step(cache_idx) => { Evict_Refines(s, s', op, cache_idx); }
+      case ProcessRead_Step(disk_idx) => { ProcessRead_Refines(s, s', op, disk_idx); }
+      case ProcessWrite_Step(disk_idx) => { ProcessWrite_Refines(s, s', op, disk_idx); }
+      case Crash_Step => { Crash_Refines(s, s', op); }
+      case NewTicket_Step => { NewTicket_Refines(s, s', op); }
+      case ConsumeStub_Step => { ConsumeStub_Refines(s, s', op); }
+      case ApplyRead_Step(rid, cache_idx) => { ApplyRead_Refines(s, s', op, rid, cache_idx); }
+      case ApplyWrite_Step(rid, cache_idx) => { ApplyWrite_Refines(s, s', op, rid, cache_idx); }
+    }
+  }
+
+
+  lemma NextRefinesNext(s: A.Variables, s': A.Variables, op: ifc.Op)
+  //requires Inv(s)
+  //requires Inv(s')
+  //requires A.Next(s, s', op)
+  ensures B.Next(I(s), I(s'), op)
 }
